Add additional lemmas

CPL_Completeness.thy
@@ -6,6 +6,15 @@ begin
 
 (* ======================== Auxiliary Functions ======================== *)
 
+fun buildJudgementAtom :: "nat \<Rightarrow> Variable list \<Rightarrow> Relation \<Rightarrow> 'a Structure \<Rightarrow> 'a Judgement" where
+"buildJudgementAtom i var_list r \<B> = (if (wfCPLFormula (Atom r var_list) \<B>)
+    then (case ((Interp \<B>) r) of
+      None \<Rightarrow> (Judgement 0 {} {}) |
+      (Some f) \<Rightarrow> Judgement i (set var_list) (buildAtomValuations var_list f)
+    )
+    else (Judgement 0 {} {})
+)"
+
 fun join :: "'a Judgement \<Rightarrow> 'a Judgement \<Rightarrow> 'a Judgement" where
 "join \<J>\<^sub>0 \<J>\<^sub>1 = Judgement (Index \<J>\<^sub>0) ((Vars \<J>\<^sub>0) \<union> (Vars \<J>\<^sub>1)) (joinJudgementValuations \<J>\<^sub>0 \<J>\<^sub>1)"
 
@@ -21,18 +30,65 @@ fun dualProject :: "Variable \<Rightarrow> 'a Judgement \<Rightarrow> 'a Structu
 fun project :: "'a Judgement \<Rightarrow> Variable set \<Rightarrow> 'a Judgement" where
 "project \<J> V = (Judgement (Index \<J>) V (projectJudgementValuations \<J> V))"
 
+(* ======================== Auxiliary Lemmas ======================== *)
+
+lemma build_judgement_atom_can_be_null_when_interpretation_does_not_have_relation [simp] : "\<lbrakk>
+  ((Interp \<B>) r) = None
+\<rbrakk> \<Longrightarrow> (buildJudgementAtom i var_list r \<B>) = (Judgement 0 {} {})"
+  by (auto)
+
+lemma build_judgement_atom_cannot_be_null_when_interpretation_has_relation [simp] : "\<lbrakk>
+  (\<phi>\<^sub>L, P\<^sub>L) = (buildFormulaParentList \<phi>);
+  (i \<in> (setOfIndex P\<^sub>L));
+  (wfCPLFormula (Atom r var_list) \<B>);
+  ((Interp \<B>) r) = (Some f)
+\<rbrakk> \<Longrightarrow> (buildJudgementAtom i var_list r \<B>) \<noteq> (Judgement 0 {} {})"
+  by (auto)
+
+lemma build_judgement_atom_index_is_maintained [simp] : "\<lbrakk>
+  (\<phi>\<^sub>L, P\<^sub>L) = (buildFormulaParentList \<phi>);
+  (i \<in> (setOfIndex P\<^sub>L));
+  (wfCPLFormula (Atom r var_list) \<B>);
+  ((Interp \<B>) r) = (Some f)
+\<rbrakk> \<Longrightarrow> (Index (buildJudgementAtom i var_list r \<B>)) = i"
+  by (auto)
+
+lemma build_judgement_atom_index_is_defined [simp] : "\<lbrakk>
+  (\<phi>\<^sub>L, P\<^sub>L) = (buildFormulaParentList \<phi>);
+  (i \<in> (setOfIndex P\<^sub>L));
+  (wfCPLFormula (Atom r var_list) \<B>);
+  ((Interp \<B>) r) = (Some f)
+\<rbrakk> \<Longrightarrow> (Vars (buildJudgementAtom i var_list r \<B>)) = (set var_list)"
+  by (auto)
+
+lemma join_index_is_maintained [simp] : "(Index (join \<J>\<^sub>0 \<J>\<^sub>1)) = (Index \<J>\<^sub>0)"
+  by (auto)
+
+lemma join_var_set_is_increased [simp] : "(Vars (join \<J>\<^sub>0 \<J>\<^sub>1)) = ((Vars \<J>\<^sub>0) \<union> (Vars \<J>\<^sub>1))"
+  by (auto)
+
+lemma dual_project_index_is_maintained [simp] : "(Index (dualProject y \<J> \<B>)) = (Index \<J>)"
+  apply (auto)
+  by (meson Judgement.sel(1))
+
+lemma dual_project_var_set_is_reduced [simp] : "(Vars (dualProject y \<J> \<B>)) = ((Vars \<J>) - {y})"
+  apply (auto)
+  apply (metis Diff_iff Judgement.sel(2))
+  apply (metis DiffE Judgement.sel(2) insertCI)
+  by (metis DiffI Judgement.sel(2) singletonD)
+
+lemma project_var_set_is_maintained [simp] : "(Vars (project \<J> V)) = V"
+  by (auto)
+
 (* ======================== Canonical Judgement Functions ======================== *)
 
 function canonicalJudgementRec :: "Formula \<Rightarrow> nat \<Rightarrow> Formula list \<Rightarrow> ParentIndex list \<Rightarrow> 'a Structure \<Rightarrow> 'a Judgement" where
-"(((length \<phi>\<^sub>L) = 0) \<or> (i = 0)) \<Longrightarrow> canonicalJudgementRec \<psi> i \<phi>\<^sub>L P\<^sub>L \<B> = (Judgement 0 {} {})" |
-"((length \<phi>\<^sub>L) > 0) \<and> (i > (length \<phi>\<^sub>L)) \<Longrightarrow> canonicalJudgementRec \<psi> i \<phi>\<^sub>L P\<^sub>L \<B> = (Judgement 0 {} {})" |
-"((length \<phi>\<^sub>L) > 0) \<and> (i > 0) \<and> (i \<le> (length \<phi>\<^sub>L)) \<Longrightarrow> canonicalJudgementRec \<psi> i \<phi>\<^sub>L P\<^sub>L \<B> = (
+"((\<not> (wfCPLFormula \<psi> \<B>)) \<or> ((length P\<^sub>L) = 0) \<or> (i = 0)) \<Longrightarrow> canonicalJudgementRec \<psi> i \<phi>\<^sub>L P\<^sub>L \<B> = (Judgement 0 {} {})" |
+"(wfCPLFormula \<psi> \<B>) \<and> ((length P\<^sub>L) > 0) \<and> (i > (length P\<^sub>L)) \<Longrightarrow> canonicalJudgementRec \<psi> i \<phi>\<^sub>L P\<^sub>L \<B> = (Judgement 0 {} {})" |
+"(wfCPLFormula \<psi> \<B>) \<and> ((length P\<^sub>L) > 0) \<and> (i > 0) \<and> (i \<le> (length P\<^sub>L)) \<Longrightarrow> canonicalJudgementRec \<psi> i \<phi>\<^sub>L P\<^sub>L \<B> = (
   case \<psi> of
-  (Atom r var_list) \<Rightarrow> (let
-      \<I> = (Interp \<B>)
-    in (
-      Judgement i (set var_list) (buildAtomValuations var_list (the (\<I> r)))
-    )
+  (Atom r var_list) \<Rightarrow> (
+    buildJudgementAtom i var_list r \<B>
   ) |
   (Forall x \<psi>\<^sub>1) \<Rightarrow> (let
     \<J>\<^sub>0 = (canonicalJudgementRec \<psi>\<^sub>1 (i+1) \<phi>\<^sub>L P\<^sub>L \<B>)
@@ -69,18 +125,17 @@ function canonicalJudgementRec :: "Formula \<Rightarrow> nat \<Rightarrow> Formu
   using linorder_not_less by blast
 termination canonicalJudgementRec
   apply (relation "measures [\<lambda>(\<psi>, _, _, _, _). formulaDepth \<psi>]")
-  apply (auto)
-  done
+  by (auto)
 
 fun canonicalJudgement :: "nat \<Rightarrow> Formula \<Rightarrow> 'a Structure \<Rightarrow> 'a Judgement" where
 "canonicalJudgement 0 \<phi> \<B> = (Judgement 0 {} {})" |
 "canonicalJudgement i \<phi> \<B> = (let
     (\<phi>\<^sub>L, P\<^sub>L) = buildFormulaParentList \<phi>
   in (
-    (if ((i = 0) \<or> (i > (length \<phi>\<^sub>L)) \<or> ((length \<phi>\<^sub>L) = 0))
+    (if ((\<not> (wfCPLFormula \<phi> \<B>)) \<or> (i = 0) \<or> (i > (length P\<^sub>L)) \<or> ((length P\<^sub>L) = 0))
       then (Judgement 0 {} {})
       else (canonicalJudgementRec (FoI i \<phi>\<^sub>L) i \<phi>\<^sub>L P\<^sub>L \<B>)
-    )                      
+    )
   )
 )"
 
@@ -90,6 +145,48 @@ fun setOfValModels :: "Formula \<Rightarrow> 'a Structure \<Rightarrow> 'a Valua
 *)
 
 (* ======================== Canonical Judgement Lemmas ======================== *)
+
+(*
+lemma canonical_judgement_rec_cannot_be_null_judgement_if_valid [simp] : "\<lbrakk>
+  (\<phi>\<^sub>L, P\<^sub>L) = (buildFormulaParentList \<phi>);
+  (i \<in> (setOfIndex P\<^sub>L));
+  ((length P\<^sub>L) > 0);
+  (i > 0);
+  (i \<le> (length P\<^sub>L));
+  \<psi> = (FoI i \<phi>\<^sub>L)
+\<rbrakk> \<Longrightarrow> (canonicalJudgementRec \<psi> i \<phi>\<^sub>L P\<^sub>L \<B>) \<noteq> (Judgement 0 {} {})"
+  apply (auto)
+*)
+
+lemma canonical_judgement_rec_index_is_maintained_for_atom [simp] :
+  fixes \<phi> :: Formula
+  fixes \<B> :: "'a Structure"
+  fixes i :: nat
+  fixes \<J>\<^sub>c :: "'a Judgement"
+  fixes \<phi>\<^sub>L :: "Formula list"
+  fixes P\<^sub>L :: "nat list"
+  fixes r :: Relation
+  fixes var_list :: "Variable list"
+  assumes "(wfCPLInstance \<phi> \<B>)"
+  assumes "(\<phi>\<^sub>L, P\<^sub>L) = (buildFormulaParentList \<phi>)"
+  assumes "(i \<in> (setOfIndex P\<^sub>L))"
+  assumes "(Atom r var_list) = (FoI i \<phi>\<^sub>L)"
+  shows "(Index (canonicalJudgementRec (Atom r var_list) i \<phi>\<^sub>L P\<^sub>L \<B>)) = i"
+proof -
+  obtain \<psi> where "\<psi> = (FoI i \<phi>\<^sub>L)" by auto
+  have "isFormulaAtom \<psi>" by (metis \<open>\<psi> = FoI i \<phi>\<^sub>L\<close> assms(4) isFormulaAtom.simps(1)) 
+  have "((length P\<^sub>L) > 0)" using assms(2) parent_list_is_never_empty by auto
+  have "(length \<phi>\<^sub>L) = (length P\<^sub>L)" by (metis assms(2) formula_and_parent_list_are_always_the_same_length fst_conv snd_conv)
+  have "(i > 0) \<and> (i \<le> (length P\<^sub>L))" using Suc_le_eq assms(3) by auto
+  have "(wfCPLFormula \<phi> \<B>)" using assms(1) by auto
+  have "(wfFormula \<phi> (Sig \<B>))" using assms(1) by auto
+  have "(wfFormula \<psi> (Sig \<B>))" by (metis \<open>\<psi> = FoI i \<phi>\<^sub>L\<close> \<open>wfCPLFormula \<phi> \<B>\<close> assms(2) assms(3) foi_index_is_well_formed_if_root_formula_is_well_formed fst_conv wfCPLFormula.elims(1)) 
+  have "((Interp \<B>) r) \<noteq> None" by (metis \<open>\<psi> = FoI i \<phi>\<^sub>L\<close> \<open>wfCPLFormula \<phi> \<B>\<close> \<open>wfFormula \<psi> (Sig \<B>)\<close> assms(4) wfCPLFormula.elims(2) wfCPLFormula.elims(3) wf_atom_in_wf_structure_always_has_an_interpretation_for_its_relation) 
+  obtain \<J> where "\<J> = (canonicalJudgementRec \<psi> i \<phi>\<^sub>L P\<^sub>L \<B>)" by simp
+  have "(Index \<J>) \<noteq> 0" sorry
+  thus ?thesis sorry
+qed
+
 
 lemma canonical_judgement_is_always_well_formed [simp] : 
   fixes \<phi> :: Formula
@@ -106,6 +203,19 @@ lemma canonical_judgement_is_always_well_formed [simp] :
 proof -
   obtain \<psi> where "\<psi> = (FoI i \<phi>\<^sub>L)" by simp
   thus ?thesis sorry
+  (*proof (cases \<psi>)
+    case (Atom r var_list)
+    thus ?thesis sorry
+  next
+    case (And \<psi>\<^sub>1 \<psi>\<^sub>2)
+    then show ?thesis sorry
+  next
+    case (Forall x \<psi>\<^sub>1)
+    then show ?thesis sorry
+  next
+    case (Exists x \<psi>\<^sub>1)
+    then show ?thesis sorry
+  qed*)
 qed
 
 lemma canonical_judgement_lemma_index [simp] :
@@ -122,20 +232,23 @@ lemma canonical_judgement_lemma_index [simp] :
   shows "(Index \<J>\<^sub>c) = i"
 proof -
   obtain \<psi> where "\<psi> = (FoI i \<phi>\<^sub>L)" by simp
-  thus ?thesis sorry
-  (*proof (cases \<psi>)
+  thus ?thesis
+  proof (cases \<psi>)
     case (Atom r var_list)
+    have "i > 0 \<and> i \<le> (length P\<^sub>L)" using Suc_le_eq assms(3) by auto
+    have "(length \<phi>\<^sub>L) > 0" using assms(2) formula_list_is_never_empty by auto
+    obtain \<J> where "\<J> = canonicalJudgementRec \<psi> i \<phi>\<^sub>L P\<^sub>L \<B>" by simp
     thus ?thesis sorry
   next
     case (And \<psi>\<^sub>1 \<psi>\<^sub>2)
-    then show ?thesis sorry
+    thus ?thesis sorry
   next
     case (Forall x \<psi>\<^sub>1)
-    then show ?thesis sorry
+    thus ?thesis sorry
   next
     case (Exists x \<psi>\<^sub>1)
-    then show ?thesis sorry
-  qed*)
+    thus ?thesis sorry
+  qed
 qed
 
 lemma canonical_judgement_lemma_var_set [simp] :
@@ -190,13 +303,13 @@ proof -
     thus ?thesis sorry
   next
     case (And \<psi>\<^sub>1 \<psi>\<^sub>2)
-    then show ?thesis sorry
+    thus ?thesis sorry
   next
     case (Forall x \<psi>\<^sub>1)
-    then show ?thesis sorry
+    thus ?thesis sorry
   next
     case (Exists x \<psi>\<^sub>1)
-    then show ?thesis sorry
+    thus ?thesis sorry
   qed*)
 qed
 *)
@@ -221,13 +334,13 @@ proof -
     thus ?thesis sorry
   next
     case (And \<psi>\<^sub>1 \<psi>\<^sub>2)
-    then show ?thesis sorry
+    thus ?thesis sorry
   next
     case (Forall x \<psi>\<^sub>1)
-    then show ?thesis sorry
+    thus ?thesis sorry
   next
     case (Exists x \<psi>\<^sub>1)
-    then show ?thesis sorry
+    thus ?thesis sorry
   qed*)
 qed
 
@@ -241,14 +354,12 @@ theorem CPL_Completeness_Theorem [simp] :
   shows "isDerivable \<phi> \<B> (Judgement 1 {} {})"
 proof -
   have "(wfStructure \<B>)" using assms(1) by auto 
-  have "(wfFormula \<phi> (Sig \<B>))" using assms(1) by auto 
+  have "(wfFormula \<phi> (Sig \<B>))" using assms(1) by auto
   have "((ran e) \<subseteq> (Univ \<B>))" by simp
   have "sentence \<phi>" using assms(1) by auto
-  let ?formulaParentList = "buildFormulaParentList \<phi>"
-  obtain \<phi>\<^sub>L where "\<phi>\<^sub>L = fst ?formulaParentList" by simp
-  have "\<phi> = (FoI 1 \<phi>\<^sub>L)" by (metis \<open>\<phi>\<^sub>L = fst (buildFormulaParentList \<phi>)\<close> eq_fst_iff foi_first_index_is_always_the_root_formula) 
-  obtain P\<^sub>L where "P\<^sub>L = snd ?formulaParentList" by simp
-  have "(1 \<in> (setOfIndex P\<^sub>L))" using \<open>P\<^sub>L = snd (buildFormulaParentList \<phi>)\<close> one_is_always_in_set_of_index prod.collapse by blast
+  obtain \<phi>\<^sub>L P\<^sub>L where "(\<phi>\<^sub>L, P\<^sub>L)= (buildFormulaParentList \<phi>)" by (metis old.prod.exhaust)
+  have "\<phi> = (FoI 1 \<phi>\<^sub>L)" by (metis \<open>(\<phi>\<^sub>L, P\<^sub>L) = buildFormulaParentList \<phi>\<close> foi_first_index_is_always_the_root_formula fst_conv)
+  have "(1 \<in> (setOfIndex P\<^sub>L))" using \<open>(\<phi>\<^sub>L, P\<^sub>L) = buildFormulaParentList \<phi>\<close> one_is_always_in_set_of_index by blast
   thus ?thesis
   proof (cases \<phi>)
     case (Atom r var_list)
@@ -278,9 +389,9 @@ proof -
         case True \<comment> \<open> Note: I have made the assumption that we accept relationship symbols with arity=0 \<close>
         have "(length var_list) = 0" using \<open>sentence \<phi>\<close> \<open>set var_list = freeVar \<phi>\<close> by auto
         obtain \<J>\<^sub>c where "\<J>\<^sub>c = canonicalJudgement 1 \<phi> \<B>" by auto
-        then have "isDerivable \<phi> \<B> \<J>\<^sub>c" using \<open>1 \<in> setOfIndex P\<^sub>L\<close> \<open>P\<^sub>L = snd (buildFormulaParentList \<phi>)\<close> assms(1) canonical_judgement_lemma_is_derivable prod.collapse by blast
-        have "(Index \<J>\<^sub>c) = 1" using \<open>1 \<in> setOfIndex P\<^sub>L\<close> \<open>P\<^sub>L = snd (buildFormulaParentList \<phi>)\<close> \<open>\<J>\<^sub>c = canonicalJudgement 1 \<phi> \<B>\<close> assms(1) canonical_judgement_lemma_index by blast 
-        have "(Vars \<J>\<^sub>c) = {}" by (metis \<open>1 \<in> setOfIndex P\<^sub>L\<close> \<open>P\<^sub>L = snd (buildFormulaParentList \<phi>)\<close> \<open>\<J>\<^sub>c = canonicalJudgement 1 \<phi> \<B>\<close> \<open>\<phi> = FoI 1 \<phi>\<^sub>L\<close> \<open>\<phi>\<^sub>L = fst (buildFormulaParentList \<phi>)\<close> \<open>freeVar \<phi> \<subseteq> dom (\<lambda>x. None)\<close> assms(1) bot.extremum_uniqueI canonical_judgement_lemma_var_set dom_empty prod.exhaust_sel) 
+        then have "isDerivable \<phi> \<B> \<J>\<^sub>c" using \<open>(\<phi>\<^sub>L, P\<^sub>L) = buildFormulaParentList \<phi>\<close> \<open>1 \<in> setOfIndex P\<^sub>L\<close> assms(1) canonical_judgement_lemma_is_derivable by blast
+        have "(Index \<J>\<^sub>c) = 1" using \<open>(\<phi>\<^sub>L, P\<^sub>L) = buildFormulaParentList \<phi>\<close> \<open>1 \<in> setOfIndex P\<^sub>L\<close> \<open>\<J>\<^sub>c = canonicalJudgement 1 \<phi> \<B>\<close> assms(1) canonical_judgement_lemma_index by blast 
+        have "(Vars \<J>\<^sub>c) = {}" by (metis \<open>(\<phi>\<^sub>L, P\<^sub>L) = buildFormulaParentList \<phi>\<close> \<open>1 \<in> setOfIndex P\<^sub>L\<close> \<open>\<J>\<^sub>c = canonicalJudgement 1 \<phi> \<B>\<close> \<open>\<phi> = FoI 1 \<phi>\<^sub>L\<close> \<open>sentence \<phi>\<close> assms(1) canonical_judgement_lemma_var_set sentence.elims(2)) 
         have "(Funcs \<J>\<^sub>c) = {}" sorry
         have "\<J>\<^sub>c = (Judgement 1 {} {})" by (metis Judgement.collapse \<open>Funcs \<J>\<^sub>c = {}\<close> \<open>Index \<J>\<^sub>c = 1\<close> \<open>Vars \<J>\<^sub>c = {}\<close>) 
         thus ?thesis using \<open>isDerivable \<phi> \<B> \<J>\<^sub>c\<close> by blast
@@ -289,27 +400,27 @@ proof -
   next
     case (And \<psi>\<^sub>1 \<psi>\<^sub>2)
     obtain \<J>\<^sub>c where "\<J>\<^sub>c = canonicalJudgement 1 \<phi> \<B>" by auto
-    then have "isDerivable \<phi> \<B> \<J>\<^sub>c" using \<open>1 \<in> setOfIndex P\<^sub>L\<close> \<open>P\<^sub>L = snd (buildFormulaParentList \<phi>)\<close> assms(1) canonical_judgement_lemma_is_derivable prod.collapse by blast
-    have "(Index \<J>\<^sub>c) = 1" using \<open>1 \<in> setOfIndex P\<^sub>L\<close> \<open>P\<^sub>L = snd (buildFormulaParentList \<phi>)\<close> \<open>\<J>\<^sub>c = canonicalJudgement 1 \<phi> \<B>\<close> assms(1) canonical_judgement_lemma_index by blast 
-    have "(Vars \<J>\<^sub>c) = {}" by (metis \<open>1 \<in> setOfIndex P\<^sub>L\<close> \<open>P\<^sub>L = snd (buildFormulaParentList \<phi>)\<close> \<open>\<J>\<^sub>c = canonicalJudgement 1 \<phi> \<B>\<close> \<open>\<phi> = FoI 1 \<phi>\<^sub>L\<close> \<open>\<phi>\<^sub>L = fst (buildFormulaParentList \<phi>)\<close> \<open>sentence \<phi>\<close> assms(1) canonical_judgement_lemma_var_set prod.collapse sentence.elims(2)) 
+    then have "isDerivable \<phi> \<B> \<J>\<^sub>c" using \<open>(\<phi>\<^sub>L, P\<^sub>L) = buildFormulaParentList \<phi>\<close> \<open>1 \<in> setOfIndex P\<^sub>L\<close> assms(1) canonical_judgement_lemma_is_derivable by blast
+    have "(Index \<J>\<^sub>c) = 1" using \<open>(\<phi>\<^sub>L, P\<^sub>L) = buildFormulaParentList \<phi>\<close> \<open>1 \<in> setOfIndex P\<^sub>L\<close> \<open>\<J>\<^sub>c = canonicalJudgement 1 \<phi> \<B>\<close> assms(1) canonical_judgement_lemma_index by blast
+    have "(Vars \<J>\<^sub>c) = {}" by (metis \<open>(\<phi>\<^sub>L, P\<^sub>L) = buildFormulaParentList \<phi>\<close> \<open>1 \<in> setOfIndex P\<^sub>L\<close> \<open>\<J>\<^sub>c = canonicalJudgement 1 \<phi> \<B>\<close> \<open>\<phi> = FoI 1 \<phi>\<^sub>L\<close> \<open>sentence \<phi>\<close> assms(1) canonical_judgement_lemma_var_set sentence.elims(2)) 
     have "(Funcs \<J>\<^sub>c) = {}" sorry
     have "\<J>\<^sub>c = (Judgement 1 {} {})" by (metis Judgement.collapse \<open>Funcs \<J>\<^sub>c = {}\<close> \<open>Index \<J>\<^sub>c = 1\<close> \<open>Vars \<J>\<^sub>c = {}\<close>) 
     thus ?thesis using \<open>isDerivable \<phi> \<B> \<J>\<^sub>c\<close> by auto
   next
     case (Forall x \<psi>)
     obtain \<J>\<^sub>c where "\<J>\<^sub>c = canonicalJudgement 1 \<phi> \<B>" by auto
-    then have "isDerivable \<phi> \<B> \<J>\<^sub>c" using \<open>1 \<in> setOfIndex P\<^sub>L\<close> \<open>P\<^sub>L = snd (buildFormulaParentList \<phi>)\<close> assms(1) canonical_judgement_lemma_is_derivable prod.collapse by blast 
-    have "(Index \<J>\<^sub>c) = 1" using \<open>1 \<in> setOfIndex P\<^sub>L\<close> \<open>P\<^sub>L = snd (buildFormulaParentList \<phi>)\<close> \<open>\<J>\<^sub>c = canonicalJudgement 1 \<phi> \<B>\<close> assms(1) canonical_judgement_lemma_index by blast 
-    have "(Vars \<J>\<^sub>c) = {}" by (metis \<open>1 \<in> setOfIndex P\<^sub>L\<close> \<open>P\<^sub>L = snd (buildFormulaParentList \<phi>)\<close> \<open>\<J>\<^sub>c = canonicalJudgement 1 \<phi> \<B>\<close> \<open>\<phi> = FoI 1 \<phi>\<^sub>L\<close> \<open>\<phi>\<^sub>L = fst (buildFormulaParentList \<phi>)\<close> \<open>sentence \<phi>\<close> assms(1) canonical_judgement_lemma_var_set prod.collapse sentence.elims(2)) 
+    then have "isDerivable \<phi> \<B> \<J>\<^sub>c" using \<open>(\<phi>\<^sub>L, P\<^sub>L) = buildFormulaParentList \<phi>\<close> \<open>1 \<in> setOfIndex P\<^sub>L\<close> assms(1) canonical_judgement_lemma_is_derivable by blast 
+    have "(Index \<J>\<^sub>c) = 1" using \<open>(\<phi>\<^sub>L, P\<^sub>L) = buildFormulaParentList \<phi>\<close> \<open>1 \<in> setOfIndex P\<^sub>L\<close> \<open>\<J>\<^sub>c = canonicalJudgement 1 \<phi> \<B>\<close> assms(1) canonical_judgement_lemma_index by blast 
+    have "(Vars \<J>\<^sub>c) = {}" by (metis \<open>(\<phi>\<^sub>L, P\<^sub>L) = buildFormulaParentList \<phi>\<close> \<open>1 \<in> setOfIndex P\<^sub>L\<close> \<open>\<J>\<^sub>c = canonicalJudgement 1 \<phi> \<B>\<close> \<open>\<phi> = FoI 1 \<phi>\<^sub>L\<close> \<open>sentence \<phi>\<close> assms(1) canonical_judgement_lemma_var_set sentence.elims(2))
     have "(Funcs \<J>\<^sub>c) = {}" sorry
     have "\<J>\<^sub>c = (Judgement 1 {} {})" by (metis Judgement.collapse \<open>Funcs \<J>\<^sub>c = {}\<close> \<open>Index \<J>\<^sub>c = 1\<close> \<open>Vars \<J>\<^sub>c = {}\<close>) 
     thus ?thesis using \<open>isDerivable \<phi> \<B> \<J>\<^sub>c\<close> by auto  
   next
     case (Exists x \<psi>)
     obtain \<J>\<^sub>c where "\<J>\<^sub>c = canonicalJudgement 1 \<phi> \<B>" by auto
-    then have "isDerivable \<phi> \<B> \<J>\<^sub>c" using \<open>1 \<in> setOfIndex P\<^sub>L\<close> \<open>P\<^sub>L = snd (buildFormulaParentList \<phi>)\<close> assms(1) canonical_judgement_lemma_is_derivable prod.collapse by blast 
-    have "(Index \<J>\<^sub>c) = 1" using \<open>1 \<in> setOfIndex P\<^sub>L\<close> \<open>P\<^sub>L = snd (buildFormulaParentList \<phi>)\<close> \<open>\<J>\<^sub>c = canonicalJudgement 1 \<phi> \<B>\<close> assms(1) canonical_judgement_lemma_index by blast
-    have "(Vars \<J>\<^sub>c) = {}" by (metis \<open>1 \<in> setOfIndex P\<^sub>L\<close> \<open>P\<^sub>L = snd (buildFormulaParentList \<phi>)\<close> \<open>\<J>\<^sub>c = canonicalJudgement 1 \<phi> \<B>\<close> \<open>\<phi> = FoI 1 \<phi>\<^sub>L\<close> \<open>\<phi>\<^sub>L = fst (buildFormulaParentList \<phi>)\<close> \<open>sentence \<phi>\<close> assms(1) canonical_judgement_lemma_var_set prod.collapse sentence.elims(2)) 
+    then have "isDerivable \<phi> \<B> \<J>\<^sub>c" using \<open>(\<phi>\<^sub>L, P\<^sub>L) = buildFormulaParentList \<phi>\<close> \<open>1 \<in> setOfIndex P\<^sub>L\<close> assms(1) canonical_judgement_lemma_is_derivable by blast 
+    have "(Index \<J>\<^sub>c) = 1" using \<open>(\<phi>\<^sub>L, P\<^sub>L) = buildFormulaParentList \<phi>\<close> \<open>1 \<in> setOfIndex P\<^sub>L\<close> \<open>\<J>\<^sub>c = canonicalJudgement 1 \<phi> \<B>\<close> assms(1) canonical_judgement_lemma_index by blast 
+    have "(Vars \<J>\<^sub>c) = {}" using \<open>(\<phi>\<^sub>L, P\<^sub>L) = buildFormulaParentList \<phi>\<close> \<open>1 \<in> setOfIndex P\<^sub>L\<close> \<open>\<J>\<^sub>c = canonicalJudgement 1 \<phi> \<B>\<close> \<open>\<phi> = FoI 1 \<phi>\<^sub>L\<close> \<open>sentence \<phi>\<close> assms(1) canonical_judgement_lemma_var_set sentence.simps by blast 
     have "(Funcs \<J>\<^sub>c) = {}" sorry
     have "\<J>\<^sub>c = (Judgement 1 {} {})" by (metis Judgement.collapse \<open>Funcs \<J>\<^sub>c = {}\<close> \<open>Index \<J>\<^sub>c = 1\<close> \<open>Vars \<J>\<^sub>c = {}\<close>) 
     thus ?thesis using \<open>isDerivable \<phi> \<B> \<J>\<^sub>c\<close> by auto
